work on union_insert

coq/tr/left/insert.v
@@ -1,9 +1,25 @@
+(*
+
+   x |> inr X    = inr ({x} union X) 
+   x |> inl SELF = inr {x} 
+
+Note : It might seem that SELF is not needed since 
+     x |> inr{}    = inr {x} 
+However, when this is used in a semigroup-left-transform with 
+union as addition, we need SELF as the additive annihilator 
+(the most preferred set of next hops). 
+But {} is the additive identity!  (the worst set of next hops) 
+
+*) 
+
 Require Import CAS.coq.common.compute.
 Require Import CAS.coq.common.ast.
 Require Import CAS.coq.eqv.properties.
 Require Import CAS.coq.eqv.structures.
 Require Import CAS.coq.eqv.theory.
+Require Import CAS.coq.eqv.add_constant. 
 Require Import CAS.coq.eqv.set.
+Require Import CAS.coq.eqv.sum.
 Require Import CAS.coq.theory.set. 
 Require Import CAS.coq.sg.properties. 
 Require Import CAS.coq.sg.union.
@@ -16,11 +32,14 @@ Open Scope list.
 
 Section Compute.
 
-Definition ltr_insert {S : Type} (eq : brel S): ltr_type S (finite_set S) :=
-    λ x y,  bop_union eq (x :: nil) y. 
+Definition ltr_insert {S : Type} (eq : brel S): ltr_type S (with_constant (finite_set S)) :=
+  λ x y,
+  match y with
+  | inl _ => inr (x :: nil)
+  | inr X => inr (bop_union eq (x :: nil) X)
+  end.
 
 End Compute.   
-
 
 Section Theory.
 
@@ -33,57 +52,102 @@ Section Theory.
   Variable sym : brel_symmetric S eq.
   Variable trn : brel_transitive S eq. 
 
- Lemma ltr_insert_congruence : ltr_congruence S (finite_set S) eq (brel_set eq) (ltr_insert eq). 
- Proof. intros s1 s2 l1 l2 H1 H2.
-        unfold ltr_insert.
-        assert (H3 : brel_set eq (s1 :: nil) (s2 :: nil) = true). compute. rewrite H1.
-        apply sym in H1. rewrite H1. reflexivity. 
-        exact (bop_union_congruence S eq ref sym trn _ _ _ _ H3 H2). 
+  Lemma ltr_insert_congruence :
+    ltr_congruence S
+                   (with_constant (finite_set S))
+                   eq
+                   (brel_sum brel_constant (brel_set eq))
+                   (ltr_insert eq). 
+  Proof. intros s1 s2 [c1 | X1] [c2 | X2] H1 H2; simpl. 
+         + compute. rewrite H1. apply sym in H1. rewrite H1. reflexivity. 
+         + compute in H2. discriminate H2. 
+         + compute in H2. discriminate H2. 
+         + assert (H3 : brel_set eq (s1 :: nil) (s2 :: nil) = true). compute. rewrite H1.
+           apply sym in H1. rewrite H1. reflexivity. 
+           exact (bop_union_congruence S eq ref sym trn _ _ _ _ H3 H2). 
  Qed.
 
+  Lemma ltr_insert_not_left_cancellative :
+    ltr_not_left_cancellative S
+                              (with_constant (finite_set S))                              
+                              (brel_sum brel_constant (brel_set eq))
+                              (ltr_insert eq). 
+  Proof. unfold ltr_left_cancellative.
+         exists (wS, (inr nil, inr (wS::nil))); simpl.  split.
+         + apply brel_set_intro_prop; auto. split.
+           ++ intros a A.
+              apply in_set_bop_union_elim in A; auto.
+              destruct A as [A | A].
+              +++ apply in_set_singleton_elim in A; auto. 
+                  apply in_set_bop_union_intro; auto.
+                  left. compute. apply sym in A. rewrite A.
+                  reflexivity. 
+              +++ compute in A. discriminate A. 
+           ++ intros a A.
+              apply in_set_bop_union_elim in A; auto.
+              destruct A as [A | A].
+              +++ apply in_set_singleton_elim in A; auto. 
+                  apply in_set_bop_union_intro; auto.
+                  left. compute. apply sym in A. rewrite A.
+                  reflexivity. 
+              +++ apply in_set_singleton_elim in A; auto.
+                  apply in_set_bop_union_intro; auto.
+                  left. compute. apply sym in A. rewrite A.
+                  reflexivity. 
+         + compute. reflexivity. 
+Defined. 
 
- Lemma ltr_insert_not_left_cancellative : ltr_not_left_cancellative S (finite_set S) (brel_set eq) (ltr_insert eq). 
- Proof. unfold ltr_left_cancellative. exists (wS, (nil, wS::nil)). split.
-        + assert (A : ltr_insert eq wS nil = wS :: nil). compute. reflexivity. 
-          assert (B : ltr_insert eq wS (wS :: nil) = wS :: nil). compute. rewrite (ref wS). reflexivity. 
-          rewrite A, B. apply brel_set_reflexive; auto. 
-        + compute. reflexivity. 
+  Lemma ltr_insert_not_left_constant :
+    ltr_not_left_constant S
+                          (with_constant (finite_set S))                              
+                          (brel_sum brel_constant (brel_set eq))
+                          (ltr_insert eq). 
+ Proof. exists (wS, (inr nil, inr ((f wS) :: nil))).
+        destruct (nt wS) as [F1 F2]. simpl. 
+        case_eq(brel_set eq (bop_union eq (wS :: nil) nil) (bop_union eq (wS :: nil) (f wS :: nil))); intro A; auto.
+        + apply brel_set_elim_prop in A; auto.
+          destruct A as [A B].
+          assert (C : in_set eq (bop_union eq (wS :: nil) (f wS :: nil)) (f wS) = true).
+             apply in_set_bop_union_intro; auto.
+             right; compute. rewrite ref. reflexivity. 
+          assert (D := B _ C).
+          apply in_set_bop_union_elim in D; auto.
+          destruct D as [D | D].
+          ++ compute in D. rewrite F2 in D. discriminate D. 
+          ++ compute in D. discriminate D. 
  Defined.
 
-
- Lemma ltr_insert_not_left_constant : ltr_not_left_constant S (finite_set S) (brel_set eq) (ltr_insert eq). 
- Proof. exists (wS, (nil, (f wS) :: nil)).
-        destruct (nt wS) as [F1 F2]. 
-        case_eq(brel_set eq (ltr_insert eq wS nil) (ltr_insert eq wS (f wS :: nil))); intro A; auto. 
-        apply brel_set_elim_prop in A; auto.
-        destruct A as [A B].
-        assert (C : in_set eq (ltr_insert eq wS (f wS :: nil)) (f wS) = true).
-           unfold ltr_insert.
-           apply in_set_bop_union_intro; auto.
-           right. compute. rewrite ref. reflexivity. 
-        assert (D := B _ C).
-        unfold ltr_insert in D.
-        apply in_set_bop_union_elim in D; auto.
-        destruct D as [D | D]. 
-        + compute in D. rewrite F2 in D. discriminate D. 
-        + compute in D. discriminate D. 
- Defined.
+ Lemma ltr_insert_not_is_right :
+   ltr_not_is_right S
+                    (with_constant (finite_set S))                              
+                    (brel_sum brel_constant (brel_set eq))
+                    (ltr_insert eq). 
+ Proof. exists (wS, inr nil). compute; auto. Defined.
  
- Lemma ltr_insert_not_is_right : ltr_not_is_right S (finite_set S) (brel_set eq) (ltr_insert eq). 
- Proof. unfold ltr_not_is_right. exists (wS, nil). compute; auto. Defined.
- 
- Lemma ltr_insert_not_exists_id : ltr_not_exists_id S (finite_set S) (brel_set eq) (ltr_insert eq). 
- Proof. unfold ltr_not_exists_id. intro s. unfold ltr_not_is_id. exists nil. compute; auto. Defined.
+ Lemma ltr_insert_not_exists_id :
+   ltr_not_exists_id S
+                    (with_constant (finite_set S))                              
+                    (brel_sum brel_constant (brel_set eq))
+                    (ltr_insert eq). 
+ Proof. intro s. exists (inr nil). compute; auto. Defined.
 
 Lemma ltr_insert_enum_is_ann (enum : carrier_is_finite S eq) : 
-  ltr_is_ann S (finite_set S) (brel_set eq) (ltr_insert eq) ((projT1 enum) tt).
+  ltr_is_ann S
+             (with_constant (finite_set S))                              
+             (brel_sum brel_constant (brel_set eq))
+             (ltr_insert eq)
+             (inr ((projT1 enum) tt)).
 Proof. assert (A := bop_union_enum_is_ann S eq ref sym trn enum).
          intro s. unfold ltr_insert.
          destruct (A (s :: nil)) as [B C]. exact C. 
 Qed. 
 
-Lemma ltr_insert_exists_ann (enum : carrier_is_finite S eq) : ltr_exists_ann S (finite_set S) (brel_set eq) (ltr_insert eq).
-Proof. exists (projT1 enum tt). apply ltr_insert_enum_is_ann. Defined.
+Lemma ltr_insert_exists_ann (enum : carrier_is_finite S eq) :
+  ltr_exists_ann S
+                 (with_constant (finite_set S))                              
+                 (brel_sum brel_constant (brel_set eq))
+                 (ltr_insert eq).
+Proof. exists (inr (projT1 enum tt)). apply ltr_insert_enum_is_ann. Defined.
 
 Lemma list_set_hack : ∀ l s,  in_set eq l s = true -> in_list eq l s = true. 
 Proof. induction l; intros s A.
@@ -95,21 +159,28 @@ Proof. induction l; intros s A.
          ++ right. apply IHl; auto. 
 Qed. 
        
-Lemma ltr_insert_not_exists_ann (nfin : carrier_is_not_finite S eq) : ltr_not_exists_ann S (finite_set S) (brel_set eq) (ltr_insert eq). 
+Lemma ltr_insert_not_exists_ann (nfin : carrier_is_not_finite S eq) :
+  ltr_not_exists_ann S
+                     (with_constant (finite_set S))                              
+                     (brel_sum brel_constant (brel_set eq))
+                     (ltr_insert eq). 
   intros s. unfold carrier_is_not_finite in nfin. 
   unfold ltr_not_is_ann. unfold ltr_insert.
-  assert (A := nfin (fun tt => s)). simpl in A.
-  destruct A as [t P].
-  exists t. 
-  case_eq(brel_set eq (bop_union eq (t :: nil) s) s); intro B; auto.
-  apply brel_set_elim_prop in B; auto. destruct B as [B C].
-  assert (D : set.in_set eq (bop_union eq (t :: nil) s) t = true).
-  apply in_set_bop_union_intro; auto. left. compute. rewrite (ref t). reflexivity. 
-  assert (E := B t D).
-  assert (F := list_set_hack s t E).
-  rewrite F in P.
-  discriminate P. 
-Qed. 
+  destruct s as [c | s].
+  + exists wS. compute. reflexivity. 
+  + assert (A := nfin (fun tt => s)). simpl in A.
+    destruct A as [t P].
+    exists t. 
+    case_eq(brel_set eq (bop_union eq (t :: nil) s) s); intro B; auto.
+    ++ apply brel_set_elim_prop in B; auto.
+       destruct B as [B C].
+       assert (D : set.in_set eq (bop_union eq (t :: nil) s) t = true).
+          apply in_set_bop_union_intro; auto. left. compute. rewrite (ref t). reflexivity. 
+       assert (E := B t D).
+       assert (F := list_set_hack s t E).
+      rewrite F in P.
+      discriminate P. 
+Defined. 
  
 End Theory.
 
@@ -123,7 +194,12 @@ Variable f : S -> S.
 Variable nt : brel_not_trivial S eq f.
 Variable eqvP : eqv_proofs S eq. 
 
-Definition ltr_insert_proofs : left_transform_proofs S (finite_set S) (brel_set eq) eq (ltr_insert eq) :=
+Definition ltr_insert_proofs :
+  left_transform_proofs S
+                        (with_constant (finite_set S))                              
+                        (brel_sum brel_constant (brel_set eq))
+                        eq
+                        (ltr_insert eq) :=
 let ref := A_eqv_reflexive _ _ eqvP in
 let sym := A_eqv_symmetric _ _ eqvP in
 let trn := A_eqv_transitive _ _ eqvP in     
@@ -131,12 +207,12 @@ let trn := A_eqv_transitive _ _ eqvP in
   A_left_transform_congruence          := ltr_insert_congruence S eq ref sym trn
 ; A_left_transform_is_right_d          := inr(ltr_insert_not_is_right S eq wS)
 ; A_left_transform_left_constant_d     := inr(ltr_insert_not_left_constant S eq wS f nt ref sym trn)                                               
-; A_left_transform_left_cancellative_d := inr(ltr_insert_not_left_cancellative S eq wS ref sym)
+; A_left_transform_left_cancellative_d := inr(ltr_insert_not_left_cancellative S eq wS ref sym trn)
 |}.
 
 End Proofs.
 
-Definition A_left_transform_insert (S : Type) (eqv : A_eqv S) :=
+Definition A_left_transform_insert (S : Type) (eqv : A_eqv S) (c : cas_constant) :=
 let eq := A_eqv_eq _ eqv in
 let wS := A_eqv_witness S eqv in
 let f  := A_eqv_new S eqv in
@@ -146,14 +222,14 @@ let ref := A_eqv_reflexive _ _ eqvP in
 let sym := A_eqv_symmetric _ _ eqvP in
 let trn := A_eqv_transitive _ _ eqvP in 
 {|
-  A_left_transform_carrier      := A_eqv_set S eqv 
+  A_left_transform_carrier      := A_eqv_add_constant _ (A_eqv_set S eqv) c 
 ; A_left_transform_label        := eqv                                                     
 ; A_left_transform_ltr          := ltr_insert eq 
 ; A_left_transform_exists_id_d  := inr(ltr_insert_not_exists_id S eq) 
 ; A_left_transform_exists_ann_d :=
                         match A_eqv_finite_d _ eqv with
                         | inl fin => inl (ltr_insert_exists_ann S eq ref sym trn fin) 
-                        | inr nfin => inr (ltr_insert_not_exists_ann S eq ref sym trn nfin)
+                        | inr nfin => inr (ltr_insert_not_exists_ann S eq wS ref sym trn nfin)
                         end 
 ; A_left_transform_proofs       := ltr_insert_proofs S eq wS f nt eqvP 
 ; A_left_transform_ast          := Ast_ltr_insert (A_eqv_ast S eqv) 
@@ -161,28 +237,26 @@ let trn := A_eqv_transitive _ _ eqvP in
 
 End ACAS.
 
-
-
 Section CAS.
 
-Definition ltr_insert_certs {S : Type} (wS : S) (f : S -> S) : @left_transform_certificates S (list S) := 
+Definition ltr_insert_certs {S : Type} (wS : S) (f : S -> S) : @left_transform_certificates S (with_constant (list S)) := 
 {|
   left_transform_congruence            := Assert_Ltr_Congruence 
-; left_transform_is_right_d            := Certify_Ltr_Not_Is_Right (wS, nil)
-; left_transform_left_constant_d       := Certify_Ltr_Not_Left_Constant (wS, (nil, (f wS) :: nil))                                                          
-; left_transform_left_cancellative_d   := Certify_Ltr_Not_Left_Cancellative (wS, (nil, wS :: nil))
+; left_transform_is_right_d            := Certify_Ltr_Not_Is_Right (wS, inr nil)
+; left_transform_left_constant_d       := Certify_Ltr_Not_Left_Constant (wS, (inr nil, inr ((f wS) :: nil)))
+; left_transform_left_cancellative_d   := Certify_Ltr_Not_Left_Cancellative (wS, (inr nil, inr (wS :: nil)))
 |}.
 
 
-Definition left_transform_insert {S : Type} (eqv : @eqv S) :=
+Definition left_transform_insert {S : Type} (eqv : @eqv S) (c : cas_constant) :=
 {|
-  left_transform_carrier      := eqv_set eqv 
+  left_transform_carrier      := eqv_add_constant (eqv_set eqv) c 
 ; left_transform_label        := eqv                                                     
 ; left_transform_ltr          := ltr_insert (eqv_eq eqv)
 ; left_transform_exists_id_d  := Certify_Ltr_Not_Exists_Id
 ; left_transform_exists_ann_d :=
                         match eqv_finite_d eqv with
-                        | Certify_Is_Finite f => Certify_Ltr_Exists_Ann (f tt) 
+                        | Certify_Is_Finite f => Certify_Ltr_Exists_Ann (inr (f tt)) 
                         | Certify_Is_Not_Finite => Certify_Ltr_Not_Exists_Ann 
                         end 
 ; left_transform_certs        := ltr_insert_certs (eqv_witness eqv) (eqv_new eqv) 
@@ -193,31 +267,34 @@ Definition left_transform_insert {S : Type} (eqv : @eqv S) :=
 End CAS. 
 Section Verify.
 
-Lemma correct_ltr_certs_insert (S : Type) (eS : A_eqv S): 
+Lemma correct_ltr_insert_certs (S : Type) (eS : A_eqv S): 
   P2C_left_transform
-          S (finite_set S)
-          (brel_set (A_eqv_eq S eS))
-          (A_eqv_eq S eS)
-          (ltr_insert (A_eqv_eq S eS))
-          (ltr_insert_proofs S
-                             (A_eqv_eq S eS)
-                             (A_eqv_witness S eS)
-                             (A_eqv_new S eS)
-                             (A_eqv_not_trivial S eS)                                                          
-                             (A_eqv_proofs S eS)
-          ) 
+    S
+    (with_constant (finite_set S))
+    (brel_sum brel_constant (brel_set (A_eqv_eq S eS)))
+    (A_eqv_eq S eS)
+    (ltr_insert (A_eqv_eq S eS))
+    (ltr_insert_proofs S
+                       (A_eqv_eq S eS)
+                       (A_eqv_witness S eS)
+                       (A_eqv_new S eS)
+                       (A_eqv_not_trivial S eS)                                                          
+                       (A_eqv_proofs S eS)
+    ) 
     =                    
     ltr_insert_certs (A_eqv_witness S eS) (A_eqv_new S eS).
-Proof. compute. reflexivity. Qed. 
+Proof. destruct eS. destruct A_eqv_proofs.
+       destruct A_eqv_finite_d; compute; reflexivity. Qed. 
 
 
-Theorem correct_left_transform_insert (S : Type) (eS : A_eqv S)  : 
-         left_transform_insert (A2C_eqv S eS) 
+Theorem correct_left_transform_insert (S : Type) (eS : A_eqv S) (c : cas_constant) : 
+         left_transform_insert (A2C_eqv S eS) c
          = 
-         A2C_left_transform S (finite_set S) (A_left_transform_insert S eS). 
+         A2C_left_transform S (with_constant (finite_set S)) (A_left_transform_insert S eS c). 
 Proof. unfold left_transform_insert, A_left_transform_insert, A2C_left_transform; simpl.
-       rewrite correct_ltr_certs_insert.        
+       rewrite correct_ltr_insert_certs.
        rewrite correct_eqv_set.
+       rewrite correct_eqv_add_constant. 
        destruct (A_eqv_finite_d S eS) as [[f P] | nfin]; simpl; 
        try reflexivity. 
 Qed. 
